Add code for skip list using arrays; replace option loc in node_rep with dummy_null; change bottom list height from 1 to 0

lazy_list/code.v
@@ -11,94 +11,67 @@ End LAZY_LIST_PARAMS.
 
 Module LazyList (Params: LAZY_LIST_PARAMS).
   Import Params.
+  
+  Definition tail : node_rep := (INT_MAX, dummy_null, None, dummy_lock).  
 
-  (* Auxiliary functions *)
-  
-  Definition find : val := 
-    rec: "find" "pred" "k" :=
-      let: "ocurr" := (nodeNext "pred") in
-      match: "ocurr" with
-        NONE => NONEV
-      | SOME "np" => 
-        let: "curr" := !"np" in
-        let: "ck" := (nodeKey "curr") in
-        if: "k" ≤ "ck"
-        then SOME ("pred", "curr")
-        else "find" "curr" "k"
-      end.
-  
-  Definition findLock : val := 
-    rec: "find" "head" "k" :=
-      let: "opair" := find "head" "k" in
-      match: "opair" with
-        NONE => NONEV
-      | SOME "pair" =>
-        let: "pred" := Fst "pair" in
-        let: "curr" := Snd "pair" in
-        acquire (nodeLock "pred");;
-        let: "onext" := (nodeNext "pred") in
-        match: "onext" with
-          NONE => NONEV
-        | SOME "np" =>
-          let: "next" := !"np" in
-          let: "nk" := (nodeKey "next") in
-          let: "ck" := (nodeKey "curr") in
-          if: "nk" = "ck" 
-          then SOME ("pred", "curr")
-          else
-            release (nodeLock "pred");;
-            "find" "pred" "k"
-        end
-      end.
-  
-  Definition dummy_lock : val := #{|loc_car := 0|}.
-  Definition tail : node_rep := (INT_MAX, None, None, dummy_lock).  
-
-  (* Lazy list creation *)
+  (* Lazy list constructor *)
   Definition new : val := 
     λ: "_", 
       let: "t" := ref (rep_to_node tail) in
-      ref (#INT_MIN, SOME "t", NONEV, newlock #()).
+      ref (#INT_MIN, "t", NONEV, newlock #()).
+
+  (* Find function *)
+  Definition find : val := 
+    rec: "find" "pred" "k" :=
+      let: "curr" := !(nodeNext "pred") in
+      let: "ck" := nodeKey "curr" in
+        if: "k" ≤ "ck"
+        then ("pred", "curr")
+        else "find" "curr" "k".
+  
+  Definition findLock : val := 
+    rec: "find" "head" "k" :=
+      let: "pair" := find "head" "k" in
+      let: "pred" := Fst "pair" in
+      let: "curr" := Snd "pair" in
+        acquire (nodeLock "pred");;
+        let: "next" := !(nodeNext "pred") in
+        let: "nk" := nodeKey "next" in
+        let: "ck" := nodeKey "curr" in
+          if: "nk" = "ck" 
+          then "pair"
+          else
+            release (nodeLock "pred");;
+            "find" "pred" "k".
 
   (* Lazy list lookup *)
   Definition contains : val := 
     λ: "head" "k",
-      let: "opair" := find !"head" "k" in
-      match: "opair" with
-        NONE => #false
-      | SOME "pair" =>
-        let: "curr" := Snd "pair" in
-        let: "ck" := (nodeKey "curr") in
-        ("k" = "ck") 
-      end.
+      let: "np" := !"head" in
+      let: "pair" := find "np" "k" in
+      let: "curr" := Snd "pair" in
+      let: "ck" := nodeKey "curr" in
+        ("k" = "ck").
   
   (* Lazy list insertion *)
   Definition add : val := 
     λ: "head" "k",
-      let: "opair" := findLock !"head" "k" in
-      match: "opair" with
-        NONE => #false
-      | SOME "pair" =>
-        let: "pred" := Fst "pair" in
-        let: "curr" := Snd "pair" in
-        let: "ck" := (nodeKey "curr") in
+      let: "np" := !"head" in
+      let: "pair" := findLock "np" "k" in
+      let: "pred" := Fst "pair" in
+      let: "curr" := Snd "pair" in
+      let: "ck" := nodeKey "curr" in
         if: "k" = "ck"
         then
           release (nodeLock "pred");;
           #false
         else
-          match: nodeNext "pred" with
-            NONE =>
-            release (nodeLock "pred");;
-            #false
-          | SOME "np" =>
-            let: "succ" := !"np" in
-            let: "next" := ref "succ" in
-            let: "node" := ("k", SOME "next", NONEV, newlock #()) in
+          let: "np" := nodeNext "pred" in
+          let: "succ" := !"np" in
+          let: "next" := ref "succ" in
+          let: "node" := ("k", "next", NONEV, newlock #()) in
             "np" <- "node";;
             release (nodeLock "pred");;
-            #true
-          end
-      end.
+            #true.
 
 End LazyList.
