lib/node_rep.v
@@ -2,10 +2,10 @@ From iris.heap_lang Require Import notation.
 
 Local Open Scope Z.
 
-Definition node_rep : Type := Z * option loc * option loc * val.
+Definition node_rep : Type := Z * loc * option loc * val.
 
 Definition node_key (n: node_rep) : Z := n.1.1.1.
-Definition node_next (n: node_rep) : option loc := n.1.1.2.
+Definition node_next (n: node_rep) : loc := n.1.1.2.
 Definition node_down (n: node_rep) : option loc := n.1.2.
 Definition node_lock (n: node_rep) : val := n.2.
 
@@ -14,6 +14,9 @@ Definition nodeNext : val := λ: "l", Snd (Fst (Fst "l")).
 Definition nodeDown : val := λ: "l", Snd (Fst "l").
 Definition nodeLock : val := λ: "l", Snd "l".
 
+Definition dummy_null : loc := {|loc_car := 0|}.
+Definition dummy_lock : val := #().
+
 Definition oloc_to_val (ol: option loc) : val := 
   match ol with
   | None => NONEV
@@ -21,11 +24,11 @@ Definition oloc_to_val (ol: option loc) : val :=
   end.
 
 Definition rep_to_node (n: node_rep) : val :=
-  (#(node_key n), oloc_to_val (node_next n), oloc_to_val (node_down n), (node_lock n)).
+  (#(node_key n), #(node_next n), oloc_to_val (node_down n), (node_lock n)).
 
 
 Lemma fold_rep_to_node (n: node_rep) :
-  ((#(node_key n), oloc_to_val (node_next n), oloc_to_val (node_down n), (node_lock n)))%V =
+  ((#(node_key n), #(node_next n), oloc_to_val (node_down n), (node_lock n)))%V =
   rep_to_node n.
 Proof. done. Qed.
 
@@ -33,9 +36,9 @@ Lemma rep_to_node_inj rep rep':
   rep_to_node rep = rep_to_node rep' →
   rep = rep'.
 Proof.
-  destruct rep as (((?&next)&down)&?). 
-  destruct rep' as (((?&next')&down')&?).
+  destruct rep as (((?&?)&down)&?). 
+  destruct rep' as (((?&?)&down')&?).
   rewrite /rep_to_node/node_key/node_next/node_down/node_lock//=.
-  destruct next; destruct next'; destruct down; destruct down'.
+  destruct down; destruct down'.
   all: inversion 1; congruence.
 Qed.
