skip_list/code.v
@@ -13,168 +13,122 @@ End SKIP_LIST_PARAMS.
 Module SkipList (Params: SKIP_LIST_PARAMS).
   Import Params.
 
-  (* 
-   * (node_down tail) is never called, so there's no problem 
-   * in having None for all levels here.
-   * The same can be said for (node_lock tail) and the dummy_lock.
-   *)
-  Definition dummy_lock : val := #().
-  Definition tail : node_rep := (INT_MAX, None, None, dummy_lock).
+  Definition tail : node_rep := (INT_MAX, dummy_null, None, dummy_lock).
 
-  (* Lazy list creation *)
+  (* Skip list constructor *)
   Definition newLoop : val := 
     rec: "loop" "head" "l" :=
       let: "h" := ref "head" in
-      if: "l" = #MAX_HEIGHT
-      then "h"
-      else
-        let: "t" := ref (rep_to_node tail) in
-        let: "head" := (#INT_MIN, SOME "t", SOME "h", newlock #()) in
-        "loop" "head" ("l" + #1).
+        if: "l" = #MAX_HEIGHT
+        then "h"
+        else
+          let: "t" := ref (rep_to_node tail) in
+          let: "head" := (#INT_MIN, "t", SOME "h", newlock #()) in
+            "loop" "head" ("l" + #1).
   
   Definition new : val := 
     λ: "_", 
       let: "t" := ref (rep_to_node tail) in
-      let: "head" := (#INT_MIN, SOME "t", NONEV, newlock #()) in
-      let: "h" := newLoop "head" #1 in
-      "h".
+      let: "head" := (#INT_MIN, "t", NONEV, newlock #()) in
+        newLoop "head" #0.
 
   (* Find function *)
   Definition find : val := 
     rec: "find" "pred" "k" :=
-      let: "ocurr" := (nodeNext "pred") in
-      match: "ocurr" with
-        NONE => NONEV
-      | SOME "np" => 
-        let: "curr" := !"np" in
-        let: "ck" := (nodeKey "curr") in
+      let: "curr" := !(nodeNext "pred") in
+      let: "ck" := nodeKey "curr" in
         if: "k" ≤ "ck"
-        then SOME ("pred", "curr")
-        else "find" "curr" "k"
-      end.
+        then ("pred", "curr")
+        else "find" "curr" "k".
   
   Definition findLock : val := 
     rec: "find" "head" "k" :=
-      let: "opair" := find "head" "k" in
-      match: "opair" with
-        NONE => NONEV
-      | SOME "pair" =>
-        let: "pred" := Fst "pair" in
-        let: "curr" := Snd "pair" in
+      let: "pair" := find "head" "k" in
+      let: "pred" := Fst "pair" in
+      let: "curr" := Snd "pair" in
         acquire (nodeLock "pred");;
-        let: "onext" := (nodeNext "pred") in
-        match: "onext" with
-          NONE => NONEV
-        | SOME "np" =>
-          let: "next" := !"np" in
-          let: "nk" := (nodeKey "next") in
-          let: "ck" := (nodeKey "curr") in
+        let: "next" := !(nodeNext "pred") in
+        let: "nk" := nodeKey "next" in
+        let: "ck" := nodeKey "curr" in
           if: "nk" = "ck" 
-          then SOME ("pred", "curr")
+          then "pair"
           else
             release (nodeLock "pred");;
-            "find" "pred" "k"
-        end
-      end.
+            "find" "pred" "k".
 
-  (* Lazy list lookup *)
+  (* Skip list lookup *)
   Definition findPred : val := 
     rec: "find" "head" "k" := 
-      let: "opair" := find "head" "k" in
-      match: "opair" with
-        NONE => NONEV
-      | SOME "pair" =>
-        let: "pred" := Fst "pair" in
-        let: "curr" := Snd "pair" in
+      let: "pair" := find "head" "k" in
+      let: "pred" := Fst "pair" in
+      let: "curr" := Snd "pair" in
         match: nodeDown "pred" with
-          NONE => SOME ("pred", "curr")
+          NONE => "pair"
         | SOME "np" => 
           let: "pred" := !"np" in
-          "find" "pred" "k"
-        end
-      end.
+            "find" "pred" "k"
+        end.
 
   Definition contains : val := 
     λ: "head" "k", 
-      let: "opair" := findPred !"head" "k" in
-      match: "opair" with
-        NONE => #false
-      | SOME "pair" => 
-        let: "curr" := Snd "pair" in
-        let: "ck" := nodeKey "curr" in
-        "k" = "ck"
-      end.
+      let: "np" := !"head" in
+      let: "pair" := findPred "np" "k" in
+      let: "curr" := Snd "pair" in
+      let: "ck" := nodeKey "curr" in
+        "k" = "ck".
 
-  (* Lazy list insertion *)
+  (* Link node in lazy list *)
   Definition link : val := 
     λ: "pred" "k" "odown",
-      match: nodeNext "pred" with
-        NONE => 
-        release (nodeLock "pred");;
-        NONEV
-      | SOME "np" =>
-        let: "succ" := !"np" in
-        let: "next" := ref "succ" in
-        let: "node" := ("k", SOME "next", "odown", newlock #()) in
+      let: "np" := nodeNext "pred" in
+      let: "succ" := !"np" in
+      let: "next" := ref "succ" in
+      let: "node" := ("k", "next", "odown", newlock #()) in
         "np" <- "node";;
         release (nodeLock "pred");;
-        SOME "node"
-      end.
+        "node".
 
+  (* Lazy list insertion *)
   Definition tryInsert : val := 
     λ: "head" "k",
-      let: "opair" := findLock "head" "k" in
-      match: "opair" with
-        NONE => NONEV
-      | SOME "pair" =>
-        let: "pred" := Fst "pair" in
-        let: "curr" := Snd "pair" in
-        let: "ck" := (nodeKey "curr") in
+      let: "pair" := findLock "head" "k" in
+      let: "pred" := Fst "pair" in
+      let: "curr" := Snd "pair" in
+      let: "ck" := (nodeKey "curr") in
         if: "k" = "ck"
         then
           release (nodeLock "pred");;
           NONEV
         else
-          link "pred" "k" NONEV
-      end.
+          let: "node" := link "pred" "k" NONEV in
+            SOME "node".
 
   Definition insert : val := 
     λ: "head" "k" "down",
-      let: "opair" := findLock "head" "k" in
-      match: "opair" with
-        NONE => NONEV
-      | SOME "pair" =>
-        let: "pred" := Fst "pair" in
-        let: "d" := ref "down" in
-        link "pred" "k" (SOME "d")
-      end.
+      let: "pair" := findLock "head" "k" in
+      let: "pred" := Fst "pair" in
+      let: "d" := ref "down" in
+        link "pred" "k" (SOME "d").
 
   (* Skip list insertion *)
   Definition topLevel : val := 
     rec: "loop" "head" "k" "h" "l" :=
-      let: "opair" := find "head" "k" in
-      match: "opair" with
-        NONE => NONEV
-      | SOME "pair" =>
-        let: "pred" := Fst "pair" in
+      let: "pair" := find "head" "k" in
+      let: "pred" := Fst "pair" in
         if: "h" = "l"
-        then SOME "pred"
+        then "pred"
         else
           match: nodeDown "pred" with
-            NONE => NONEV
+            NONE => #()
           | SOME "np" => 
             let: "pred" := !"np" in
-            "loop" "pred" "k" "h" ("l" - #1)
-          end
-      end.
+              "loop" "pred" "k" "h" ("l" - #1)
+          end.
       
   Definition addAll : val := 
     rec: "add" "head" "k" := 
-      let: "opair" := find "head" "k" in
-      match: "opair" with
-        NONE => NONEV
-      | SOME "pair" =>
-        let: "pred" := Fst "pair" in
+      let: "pair" := find "head" "k" in
+      let: "pred" := Fst "pair" in
         match: nodeDown "pred" with
           NONE => tryInsert "pred" "k"
         | SOME "np" => 
@@ -182,22 +136,20 @@ Module SkipList (Params: SKIP_LIST_PARAMS).
           let: "onode" := "add" "down" "k" in
           match: "onode" with 
             NONE => NONEV
-          | SOME "node" => insert "pred" "k" "node"
+          | SOME "node" => 
+            let: "node" := insert "pred" "k" "node" in
+              SOME "node"
           end
-        end
-      end.
+        end.
 
   Definition add : val := 
     λ: "head" "k" "h",
-      let: "opred" := topLevel !"head" "k" "h" #MAX_HEIGHT in
-      match: "opred" with
-        NONE => #false
-      | SOME "pred" => 
-        let: "onew" := addAll "pred" "k" in
-        match: "onew" with
+      let: "np" := !"head" in
+      let: "pred" := topLevel "np" "k" "h" #MAX_HEIGHT in
+      let: "onode" := addAll "pred" "k" in
+        match: "onode" with
           NONE => #false
-        | SOME "new" => #true
-        end
-      end.
+        | SOME "node" => #true
+        end.
 
 End SkipList.
