arrays/code.v
@@ -1,0 +1,147 @@
+From SkipList.lib Require Import lock node_rep.
+
+
+Local Open Scope Z.
+
+Module Type SKIP_LIST_PARAMS.
+  Parameter INT_MIN : Z.
+  Parameter INT_MAX : Z.
+  Parameter MAX_HEIGHT : Z.
+  Parameter (HMIN_MAX: INT_MIN < INT_MAX).
+End SKIP_LIST_PARAMS.
+
+Module SkipList (Params: SKIP_LIST_PARAMS).
+  Import Params.
+  
+  Definition tail : node_rep := (INT_MAX, dummy_null, None, dummy_lock).
+
+  (* Skip list constructor *)  
+  Definition new : val := 
+    λ: "_", 
+      let: "np" := ref (rep_to_node tail) in
+      let: "next" := AllocN #MAX_HEIGHT "np" in
+        ref (#INT_MIN, "next", NONEV, newlock #()).
+
+  (* Find function *)
+  Definition find : val := 
+    rec: "find" "pred" "k" "i" :=
+      let: "np" := nodeNext "pred" in
+      let: "succ" := ! !("np" +ₗ "i") in
+      let: "ck" := nodeKey "succ" in
+        if: "k" ≤ "ck"
+        then ("pred", "succ")
+        else "find" "succ" "k" "i".
+  
+  Definition findLock : val := 
+    rec: "find" "head" "k" "i" :=
+      let: "pair" := find "head" "k" "i" in
+      let: "pred" := Fst "pair" in
+      let: "curr" := Snd "pair" in
+        acquire (nodeLock "pred");;
+        let: "np" := nodeNext "pred" in
+        let: "next" := ! !("np" +ₗ "i") in
+        let: "nk" := nodeKey "next" in
+        let: "ck" := nodeKey "curr" in
+          if: "nk" = "ck" 
+          then "pair"
+          else
+            release (nodeLock "pred");;
+            "find" "pred" "k" "i".
+
+  (* Skip list lookup *)
+  Definition findPred : val := 
+    rec: "find" "pred" "k" "i" := 
+      let: "pair" := find "pred" "k" "i" in
+        if: "i" = #0
+        then "pair"
+        else 
+          let: "pred" := Fst "pair" in
+            "find" "pred" "k" ("i" - #1).
+
+  Definition contains : val := 
+    λ: "head" "k", 
+      let: "np" := !"head" in
+      let: "pair" := findPred "np" "k" #MAX_HEIGHT in
+      let: "curr" := Snd "pair" in
+      let: "ck" := nodeKey "curr" in
+        "k" = "ck".
+
+  (* Link node in lazy list *)
+  Definition createAndLink : val := 
+    λ: "pred" "k" "h",
+      let: "np" := nodeNext "pred" in
+      let: "succ" := !"np" in
+      let: "next" := AllocN "h" #() in
+      let: "node" := ref ("k", "next", NONEV, newlock #()) in
+        "next" <- "succ";;
+        "np" <- "node";;
+        "node".
+
+  Definition link : val := 
+    λ: "pred" "i" "node",
+      let: "np" := nodeNext "pred" in
+      let: "succ" := !("np" +ₗ "i") in
+      let: "next" := nodeNext !"node" in
+        ("next" +ₗ "i") <- "succ";;
+        ("np" +ₗ "i") <- "node";;
+        release (nodeLock "pred").
+
+  (* Lazy list insertion *)
+  Definition tryInsert : val := 
+    λ: "head" "k" "h",
+      let: "pair" := findLock "head" "k" #0 in
+      let: "pred" := Fst "pair" in
+      let: "curr" := Snd "pair" in
+      let: "ck" := nodeKey "curr" in
+        if: "k" = "ck"
+        then 
+          release (nodeLock "pred");;
+          NONEV
+        else 
+          let: "node" := createAndLink "pred" "k" "h" in
+            release (nodeLock "pred");;
+            SOME "node".
+
+  Definition insert : val := 
+    λ: "head" "i" "node",
+      let: "k" := nodeKey !"node" in
+      let: "pair" := findLock "head" "k" "i" in
+      let: "pred" := Fst "pair" in
+        link "pred" "i" "node";;
+        release (nodeLock "pred").
+
+  (* Skip list insertion *)
+  Definition topLevel : val := 
+    rec: "loop" "head" "k" "h" "i" :=
+      let: "pair" := find "head" "k" "i" in
+      let: "pred" := Fst "pair" in
+        if: "h" = "i"
+        then "pred"
+        else "loop" "pred" "k" "h" ("i" - #1).
+      
+  Definition addAll : val := 
+    rec: "add" "head" "k" "h" "i" := 
+      let: "pair" := find "head" "k" "i" in
+      let: "pred" := Fst "pair" in
+        if: "i" = #0
+        then tryInsert "pred" "k" "h"
+        else
+          let: "onode" := "add" "pred" "k" "h" ("i" - #1) in
+            match: "onode" with
+              NONE => NONEV
+            | SOME "node" =>
+              insert "pred" "i" "node";;
+              SOME "node"
+            end.
+
+  Definition add : val := 
+    λ: "head" "k" "h",
+      let: "np" := !"head" in
+      let: "pred" := topLevel "np" "k" "h" #MAX_HEIGHT in
+      let: "onode" := addAll "pred" "k" "h" "h" in
+        match: "onode" with
+          NONE => #false
+        | SOME "node" => #true
+        end.
+
+End SkipList.
