lazy_list/inv/list_equiv.v
@@ -26,19 +26,15 @@ Module ListEquiv (Params: LAZY_LIST_PARAMS).
       | nil => True
       | pred :: succs => 
         match succs with
-        | nil => ∃ (l: loc) (γ: gname), 
-                 ⌜ node_next pred = Some l ⌝
+        | nil => ∃ (γ: gname),
+                 node_next pred ↦{#1 / 2} rep_to_node tail
                  ∗
-                 l ↦{#1 / 2} rep_to_node tail
-                 ∗
-                 is_lock γ (node_lock pred) (node_inv l)
+                 is_lock γ (node_lock pred) (node_inv (node_next pred))
 
-        | succ :: t => ∃ (l: loc) (γ: gname), 
-                       ⌜ node_next pred = Some l ⌝
+        | succ :: t => ∃ (γ: gname),
+                       node_next pred ↦{#1 / 2} rep_to_node succ
                        ∗
-                       l ↦{#1 / 2} rep_to_node succ
-                       ∗
-                       is_lock γ (node_lock pred) (node_inv l)
+                       is_lock γ (node_lock pred) (node_inv (node_next pred))
                        ∗
                        list_equiv succs
         end
@@ -51,22 +47,20 @@ Module ListEquiv (Params: LAZY_LIST_PARAMS).
     Proof.
       destruct L as [|n].
       + iIntros "Hrep". by iFrame.
-      + iIntros "Hlist". iDestruct "Hlist" as (l γ) "(Hsome & Hpt & Hlock & Hmatch)".
+      + iIntros "Hlist". iDestruct "Hlist" as (γ) "(Hpt & Hlock & Hmatch)".
         iFrame. iIntros "Hlist". iFrame.
-        iExists l, γ. iFrame.
+        iExists γ. iFrame.
     Qed.
 
     Lemma list_equiv_split (pred succ: node_rep) (L L1 L2: list node_rep) :
       L ++ [tail] = L1 ++ [pred; succ] ++ L2 →
       list_equiv L ⊢ 
-        ∃ (l: loc) (γ: gname),
-          ⌜ node_next pred = Some l ⌝
+        ∃ (γ: gname),
+          node_next pred ↦{#1 / 2} rep_to_node succ
           ∗
-          l ↦{#1 / 2} (rep_to_node succ)
+          is_lock γ (node_lock pred) (node_inv (node_next pred))
           ∗
-          is_lock γ (node_lock pred) (node_inv l)
-          ∗
-          (l ↦{#1 / 2} (rep_to_node succ) -∗ list_equiv L).
+          (node_next pred ↦{#1 / 2} rep_to_node succ -∗ list_equiv L).
     Proof.
       revert L. induction L1 => L HL.
       + destruct L as [|curr L].
@@ -75,16 +69,16 @@ Module ListEquiv (Params: LAZY_LIST_PARAMS).
         destruct L as [|curr L].
         - inversion HL'; subst.
           iIntros "Hlist". 
-          iDestruct "Hlist" as (l γ) "(#Hsome & Hpt & #Hlock)".
-          iExists l, γ. iFrame "#"; iFrame.
+          iDestruct "Hlist" as (γ) "(Hpt & #Hlock)".
+          iExists γ. iFrame "#"; iFrame.
           iIntros "Hpt". 
-          iExists l, γ. iFrame "#"; iFrame.
+          iExists γ. iFrame "#"; iFrame.
         - inversion HL'; subst.
           iIntros "Hlist". 
-          iDestruct "Hlist" as (l γ) "(#Hsome & Hpt & #Hlock & Hmatch)".
-          iExists l, γ. iFrame "#"; iFrame.
+          iDestruct "Hlist" as (γ) "(Hpt & #Hlock & Hmatch)".
+          iExists γ. iFrame "#"; iFrame.
           iIntros "Hpt". 
-          iExists l, γ. iFrame "#"; iFrame.
+          iExists γ. iFrame "#"; iFrame.
       + destruct L as [|curr L].
         { 
           exfalso. inversion HL  as [[H0 HL']]; subst. 
@@ -102,36 +96,34 @@ Module ListEquiv (Params: LAZY_LIST_PARAMS).
         iIntros "Hlist".
         iPoseProof (list_equiv_cons with "Hlist") as "(Hlist & Himp)".
         iPoseProof (IHL1 with "Hlist") as "Hlist"; auto.
-        iDestruct "Hlist" as (l γ) "(Hsome & Hpt & Hlock & Himp')".
-        iExists l, γ. iFrame. iIntros "Hpt".
+        iDestruct "Hlist" as (γ) "(Hpt & Hlock & Himp')".
+        iExists γ. iFrame. iIntros "Hpt".
         iApply "Himp". iApply "Himp'". iFrame.
     Qed.
 
     Lemma list_equiv_invert (L: list node_rep) (head pred: node_rep) :
       pred = head ∨ In pred L →
       list_equiv ([head] ++ L) ⊢ 
-        ∃ (succ: node_rep) (l: loc) (γ: gname), 
+        ∃ (succ: node_rep) (γ: gname), 
           (⌜ In succ L ⌝ ∨ ⌜ succ = tail ⌝)
           ∗
-          ⌜ node_next pred = Some l ⌝
-          ∗
-          l ↦{#1/2} (rep_to_node succ)
+          node_next pred ↦{#1/2} rep_to_node succ
           ∗ 
-          is_lock γ (node_lock pred) (node_inv l)
+          is_lock γ (node_lock pred) (node_inv (node_next pred))
           ∗
-          (l ↦{#1/2} (rep_to_node succ) -∗ list_equiv ([head] ++ L)).
+          (node_next pred ↦{#1/2} rep_to_node succ -∗ list_equiv ([head] ++ L)).
     Proof.
       intros Hin; inversion Hin as [|Hin_L]; subst.
       + iIntros "Hlist". destruct L as [|succ' L].
-        - iDestruct "Hlist" as (l γ) "(%Hsome & Hpt & #Hlock)".
-          iExists tail, l, γ. iFrame; iFrame "#".
-          iSplit; first by iRight. iSplit; first done.
-          iIntros "Hpt". iExists l, γ.
+        - iDestruct "Hlist" as (γ) "(Hpt & #Hlock)".
+          iExists tail, γ. iFrame; iFrame "#".
+          iSplit; first by iRight.
+          iIntros "Hpt". iExists γ.
           by iFrame; iFrame "#".
-        - iDestruct "Hlist" as (l γ) "(%Hsome & Hpt & #Hlock & ?)".
-          iExists succ', l, γ. iFrame; iFrame "#".
-          iSplit; first by repeat iLeft. iSplit; first done. 
-          iIntros "Hpt". iExists l, γ.
+        - iDestruct "Hlist" as (γ) "(Hpt & #Hlock & ?)".
+          iExists succ', γ. iFrame; iFrame "#".
+          iSplit; first by repeat iLeft.
+          iIntros "Hpt". iExists γ.
           by iFrame; iFrame "#".
       + simpl in Hin_L; clear Hin.
         iIntros "Hlist".
@@ -140,23 +132,23 @@ Module ListEquiv (Params: LAZY_LIST_PARAMS).
         iInduction L as [|succ' L] "IHL"; iIntros (head) "Hin"; first by iExFalso.
         iDestruct "Hin" as "[%Heq|Hin]"; subst; iIntros "Hlist Himp".
         - destruct L as [|succ'' L]; subst.
-          * iDestruct "Hlist" as (l γ) "(%Hsome & Hpt & #Hlock)".
-            iExists tail, l, γ. iFrame; iFrame "#".
-            iSplit; first by iRight. iSplit; first done.
-            iIntros "Hpt". iApply "Himp". iExists l, γ. 
+          * iDestruct "Hlist" as (γ) "(Hpt & #Hlock)".
+            iExists tail, γ. iFrame; iFrame "#".
+            iSplit; first by iRight.
+            iIntros "Hpt". iApply "Himp". iExists γ. 
             by iFrame; iFrame "#".
-          * iDestruct "Hlist" as (l γ) "(%Hsome & Hpt & #Hlock & Hmatch)".
-            iExists succ'', l, γ. 
-            iSplit; first by iLeft; iRight; iLeft. iSplit; first done.
+          * iDestruct "Hlist" as (γ) "(Hpt & #Hlock & Hmatch)".
+            iExists succ'', γ. 
+            iSplit; first by iLeft; iRight; iLeft.
             iFrame "Hpt"; iFrame "Hlock".
             iIntros "Hpt". iApply "Himp".
-            iExists l, γ. by iFrame; iFrame "#".
+            iExists γ. by iFrame; iFrame "#".
         - iPoseProof (list_equiv_cons with "Hlist") as "(Hlist & Himp')".
           iPoseProof ("IHL" with "Hin") as "Himp''".
           iPoseProof ("Himp''" with "Hlist") as "Himp''".
           iPoseProof ("Himp''" with "Himp'") as "Hlist".
-          iDestruct "Hlist" as (succ l γ) "(Hsucc & Hsome & Hpt & Hlock & Himp')".
-          iExists succ, l, γ. iFrame; iFrame "#".
+          iDestruct "Hlist" as (succ γ) "(Hsucc & Hpt & Hlock & Himp')".
+          iExists succ, γ. iFrame; iFrame "#".
           iSplit.
           {
             iDestruct "Hsucc" as "[Hin|Heq]".
@@ -167,20 +159,20 @@ Module ListEquiv (Params: LAZY_LIST_PARAMS).
     Qed.
 
     Lemma list_equiv_insert (head pred new succ: node_rep) (L: list node_rep) 
-      (l l': loc) (γ': gname) :
+      (γ': gname) :
       node_key new < node_key tail →
       node_key pred < node_key new < node_key succ →
       Sorted node_lt ([head] ++ L ++ [tail]) →
       pred = head ∨ In pred L →
       list_equiv ([head] ++ L) ⊢ 
-        ⌜ node_next pred = Some l ⌝ ∗ l↦{#1/2} rep_to_node succ 
+        node_next pred ↦{#1/2} rep_to_node succ 
         ∗ 
-        ⌜ node_next new = Some l' ⌝ ∗ l'↦{#1/2} rep_to_node succ
+        node_next new ↦{#1/2} rep_to_node succ
         ∗
-        is_lock γ' (node_lock new) (node_inv l')
+        is_lock γ' (node_lock new) (node_inv (node_next new))
         -∗ 
           ∃ (L' L1 L2: list node_rep), 
-            l ↦ rep_to_node succ
+            node_next pred ↦ rep_to_node succ
             ∗
             ⌜ [head] ++ L ++ [tail] = L1 ++ [pred; succ] ++ L2 ⌝
             ∗
@@ -188,13 +180,13 @@ Module ListEquiv (Params: LAZY_LIST_PARAMS).
             ∗
             ⌜ Permutation ([head] ++ L') ([head; new] ++ L) ⌝ 
             ∗
-            (l ↦{#1/2} (rep_to_node new) -∗ list_equiv ([head] ++ L')).
+            (node_next pred ↦{#1/2} (rep_to_node new) -∗ list_equiv ([head] ++ L')).
     Proof.
-      iIntros (Hnew Hrange Hsort Hin) "Hlist (Hsome & Hpt & Hsome' & Hpt' & Hlock')".
+      iIntros (Hnew Hrange Hsort Hin) "Hlist (Hpt & Hpt' & Hlock')".
       remember ([head] ++ L) as L' eqn:HeqL'.
       rewrite -in_inv in Hin.
 
-      iRevert (head L HeqL' Hsort Hin) "Hlist Hsome Hpt Hsome' Hpt' Hlock'".
+      iRevert (head L HeqL' Hsort Hin) "Hlist Hpt Hpt' Hlock'".
       iInduction L' as [|pred'] "IHL'".
       { iIntros (head L Hfalse); inversion Hfalse. }
 
@@ -202,12 +194,10 @@ Module ListEquiv (Params: LAZY_LIST_PARAMS).
       inversion HeqL'; subst.
       iIntros (Hin); inversion Hin as [Heq|HinL].
       + subst.
-        iIntros "Hlist %Hsome Hpt %Hsome' Hpt' #Hlock'".
+        iIntros "Hlist Hpt Hpt' #Hlock'".
         destruct L as [|a L].
-        - iDestruct "Hlist" as (l'' γ) "(%Hsome'' & Hpt'' & #Hlock)".
-          assert (l = l'') as <- by congruence.
-          iDestruct (mapsto_agree with "Hpt Hpt''") as %Htail.
-          apply rep_to_node_inj in Htail; subst.
+        - iDestruct "Hlist" as (γ) "(Hpt'' & #Hlock)".
+          iDestruct (mapsto_agree with "Hpt Hpt''") as %Htail%rep_to_node_inj; subst.
           iExists (new :: nil), nil, nil.
           iFrame. iSplit; first done. iSplit.
           { 
@@ -215,13 +205,11 @@ Module ListEquiv (Params: LAZY_LIST_PARAMS).
             unfold node_lt; lia.
           }
           iSplit; first auto.
-          iIntros "Hpt". iExists _, _.
-          iFrame "# ∗". iSplit; first done.
-          iExists _, _. by iFrame "# ∗".
-        - iDestruct "Hlist" as (l'' γ) "(%Hsome'' & Hpt'' & #Hlock & Hmatch)".
-          assert (l = l'') as <- by congruence.
-          iDestruct (mapsto_agree with "Hpt Hpt''") as %Heq.
-          apply rep_to_node_inj in Heq; subst.
+          iIntros "Hpt". 
+          iExists γ. iFrame "# ∗".
+          iExists γ'. iFrame "#".
+        - iDestruct "Hlist" as (γ) "(Hpt'' & #Hlock & Hmatch)".
+          iDestruct (mapsto_agree with "Hpt Hpt''") as %Heq%rep_to_node_inj; subst.
           iExists (new :: a :: L), nil, (L ++ [tail]).
           iFrame. iSplit; first done. iSplit.
           { 
@@ -231,15 +219,15 @@ Module ListEquiv (Params: LAZY_LIST_PARAMS).
             all: unfold node_lt; lia.
           }
           iSplit; first auto.
-          iIntros "Hpt". iExists _, _.
-          iFrame "# ∗". iSplit; first done.
-          iExists _, _. by iFrame "# ∗".
+          iIntros "Hpt". 
+          iExists γ. iFrame "# ∗".
+          iExists γ'. iFrame "#".
       + destruct L as [|head' L]; first by inversion HinL.
-        iIntros "Hlist %Hsome Hpt %Hsome' Hpt' #Hlock'".
+        iIntros "Hlist Hpt Hpt' #Hlock'".
 
         simpl in Hsort; apply Sorted_inv in Hsort as (Hsort&Hhd).
-        iDestruct "Hlist" as (l'' γ) "(Hsome'' & Hpt'' & Hlock & Hmatch)".
-        iPoseProof ("IHL'" $! head' L with "[%] [%] [%] [$] [%] [$] [%] [$] [$]") 
+        iDestruct "Hlist" as (γ) "(Hpt'' & Hlock & Hmatch)".
+        iPoseProof ("IHL'" $! head' L with "[%] [%] [%] [$] [$] [$] [$]") 
           as "Hclose"; auto.
         
         iDestruct "Hclose" as (L' L1 L2) "(Hpt' & %Hsplit & %Hsort' & %Hperm' & Himp')".
@@ -262,7 +250,7 @@ Module ListEquiv (Params: LAZY_LIST_PARAMS).
           econstructor; econstructor.
         }
 
-        iIntros "Hpt". iExists l'', γ.
+        iIntros "Hpt". iExists γ.
         iPoseProof ("Himp'" with "Hpt") as "Hlist".
         iFrame.
     Qed.
