lazy_list/spec/contains.v
@@ -28,8 +28,8 @@ Module ContainsSpec (Params: LAZY_LIST_PARAMS).
         ∗
         ⌜ node_key curr < key < INT_MAX ⌝
       }}}
-      find (rep_to_node curr) #key
-      {{{ pred succ, RET SOMEV ((rep_to_node pred), (rep_to_node succ));
+        find (rep_to_node curr) #key
+      {{{ pred succ, RET ((rep_to_node pred), (rep_to_node succ));
         own (s_frac Γ) (◯F Skeys)
         ∗
         ⌜ key ∈ Skeys ↔ node_key succ = key ⌝
@@ -41,190 +41,170 @@ Module ContainsSpec (Params: LAZY_LIST_PARAMS).
       iIntros (curr) "Hown_frag #Hown_curr %Hrange HΦ".
       wp_lam. wp_let. wp_lam. wp_pures.
 
-      destruct (node_next curr) as [l|] eqn:Hcurr_next; wp_pures.
-      + wp_bind (Load _). 
-        iInv lazyN as (S ? L) "(>%Hperm & >%Hsort & >%Hequiv & >Hown_auth & >Hown_frac & >Hown_keys & Hlist)" "Hclose".
-        iDestruct (own_valid_2 with "Hown_frac Hown_frag") 
-          as %->%frac_auth_agree_L.
+      wp_bind (Load _). 
+      iInv lazyN as (S ? L) "(>%Hperm & >%Hsort & >%Hequiv & >Hown_auth & >Hown_frac & >Hown_keys & Hlist)" "Hclose".
+      iDestruct (own_valid_2 with "Hown_frac Hown_frag") 
+        as %->%frac_auth_agree_L.
 
-        iAssert ((⌜ curr = head ∨ In curr L ⌝)%I) with "[Hown_auth Hown_curr]" as %Hcurr_range.
+      iAssert ((⌜ curr = head ∨ In curr L ⌝)%I) with "[Hown_auth Hown_curr]" as %Hcurr_range.
+      {
+        iDestruct "Hown_curr" as "[Heq|Hown]"; first by iLeft.
+        iDestruct (own_valid_2 with "Hown_auth Hown") 
+        as %[Hvalid%gset_included]%auth_both_valid_discrete.
+        iPureIntro; right.
+        rewrite -elem_of_list_In Hperm elem_of_elements.
+        set_solver.
+      }
+
+      edestruct (in_split curr ([head] ++ L)) 
+        as (Ls&Lf&Hcurr).
+      { rewrite in_inv //. }
+
+      edestruct (node_rep_split_join Lf curr tail key) 
+        as (pred&succ&L1&L2&?&?&Hsplit_join); auto.
+      {
+        rewrite -app_ass Hcurr app_ass in Hsort.
+        apply node_rep_sorted_app in Hsort.
+        simpl in *. by destruct Hsort as [_ ?].
+      }
+
+      feed pose proof (node_rep_split_sep L Ls Lf L1 L2 head curr pred succ tail key) 
+        as Htemp; auto.
+      destruct Htemp as [Lm Hsplit_sep].
+
+      destruct Lm as [|next Lm].
+      - rewrite (list_equiv_split curr succ ([head] ++ L)); last first.
+        { rewrite app_ass -Hsplit_sep //. }
+        iDestruct "Hlist" as (γ) "(Hpt & #Hlock & Himp)".
+
+        wp_load.
+        iPoseProof ("Himp" with "Hpt") as "Hlist".
+        iMod ("Hclose" with "[Hlist Hown_auth Hown_frac Hown_keys]") as "_".
+        { iNext; iExists S, Skeys, L; by iFrame.  }
+
+        iModIntro. wp_let. wp_lam. wp_pures.
+        case_bool_decide; last lia.
+        wp_pures. iApply "HΦ".
+        iModIntro; iFrame.
+
+        iPureIntro.
+        rewrite -elem_of_elements Hequiv -Hperm.
+        split; intros.
+        * eapply (sorted_node_lt_cover_gap (Ls ++ L1) L2 pred); try lia.
+          ++ by rewrite app_ass -Hsplit_join //= app_comm_cons -app_ass -Hcurr app_ass.
+          ++ assert (In key (map node_key ([head] ++ L ++ [tail]))) as Hin.
+              { rewrite -app_ass map_app in_app_iff; left; right. 
+                by apply elem_of_list_In. }
+              rewrite -app_ass Hcurr app_ass in Hin.
+              by rewrite app_ass -Hsplit_join.
+        * rewrite elem_of_list_In in_map_iff. exists succ; split; auto.
+          cut (In succ Lf).
+          { destruct Ls; inversion Hcurr; subst; auto.
+            intros; by rewrite in_app_iff; right; right. }
+
+          cut (In succ (Lf ++ [tail])).
+          { rewrite /tail ?in_app_iff.
+            intros [|[|[]]]; auto; subst. 
+            rewrite /node_key /= in Hrange; lia. }
+
+          destruct L1.
+          ++ rewrite //= in Hsplit_join. 
+              inversion Hsplit_join as [[Heq1 Heq2]]; subst.
+              by rewrite Heq2; left.
+          ++ inversion Hsplit_join as [[Heq1 Heq2]]; subst.
+              by rewrite Heq2 in_app_iff; right; right; left.
+      - assert (next ∈ S).
         {
-         iDestruct "Hown_curr" as "[Heq|Hown]"; first by iLeft.
-         iDestruct (own_valid_2 with "Hown_auth Hown") 
-          as %[Hvalid%gset_included]%auth_both_valid_discrete.
-         iPureIntro; right.
-         rewrite -elem_of_list_In Hperm elem_of_elements.
-         set_solver.
-        }
-
-        edestruct (in_split curr ([head] ++ L)) 
-          as (Ls&Lf&Hcurr).
-        { rewrite in_inv //. }
-  
-        edestruct (node_rep_split_join Lf curr tail key) 
-          as (pred&succ&L1&L2&?&?&Hsplit_join); auto.
-        {
-          rewrite -app_ass Hcurr app_ass in Hsort.
-          apply node_rep_sorted_app in Hsort.
-          simpl in *. by destruct Hsort as [_ ?].
-        }
-  
-        feed pose proof (node_rep_split_sep L Ls Lf L1 L2 head curr pred succ tail key) 
-          as Htemp; auto.
-        destruct Htemp as [Lm Hsplit_sep].
-
-        destruct Lm as [|next Lm].
-        - rewrite (list_equiv_split curr succ ([head] ++ L)); last first.
-          { rewrite app_ass -Hsplit_sep //. }
-          iDestruct "Hlist" as (l' γ) "(>%Hsome & Hpt & #Hlock & Himp)".
-          assert (l = l') as <- by congruence.
-
-          wp_load.
-          iPoseProof ("Himp" with "Hpt") as "Hlist".
-          iMod ("Hclose" with "[Hlist Hown_auth Hown_frac Hown_keys]") as "_".
-          { iNext; iExists S, Skeys, L; by iFrame.  }
-
-          iModIntro. wp_let. wp_lam. wp_pures.
-          case_bool_decide; last lia.
-          wp_pures. iApply "HΦ".
-          iModIntro; iFrame.
-
-          iPureIntro.
-          rewrite -elem_of_elements Hequiv -Hperm.
-          split; intros.
-          * eapply (sorted_node_lt_cover_gap (Ls ++ L1) L2 pred); try lia.
-            ++ by rewrite app_ass -Hsplit_join //= app_comm_cons -app_ass -Hcurr app_ass.
-            ++ assert (In key (map node_key ([head] ++ L ++ [tail]))) as Hin.
-               { rewrite -app_ass map_app in_app_iff; left; right. 
-                 by apply elem_of_list_In. }
-               rewrite -app_ass Hcurr app_ass in Hin.
-               by rewrite app_ass -Hsplit_join.
-          * rewrite elem_of_list_In in_map_iff. exists succ; split; auto.
-            cut (In succ Lf).
-            { destruct Ls; inversion Hcurr; subst; auto.
-              intros; by rewrite in_app_iff; right; right. }
-
-            cut (In succ (Lf ++ [tail])).
-            { rewrite /tail ?in_app_iff.
-              intros [|[|[]]]; auto; subst. 
-              rewrite /node_key /= in Hrange; lia. }
-
-            destruct L1.
-            ++ rewrite //= in Hsplit_join. 
-               inversion Hsplit_join as [[Heq1 Heq2]]; subst.
-               by rewrite Heq2; left.
-            ++ inversion Hsplit_join as [[Heq1 Heq2]]; subst.
-               by rewrite Heq2 in_app_iff; right; right; left.
-        - assert (next ∈ S).
-          {
-            rewrite -elem_of_elements -Hperm.
-            destruct Ls; assert (In next (L ++ [tail])) as Hin.
-            + inversion Hsplit_sep. by left.
-            + apply in_app_iff in Hin.
-              destruct Hin as [|[|[]]]; first by eapply elem_of_list_In.
-              inversion Hsplit_sep. inversion Hcurr.
-              subst; exfalso.
-              rewrite -Hsplit_sep in Hsort.
-              do 2 apply node_rep_sorted_app in Hsort as (_ & Hsort).
-              apply Sorted_StronglySorted in Hsort; last first.
-              { unfold Relations_1.Transitive; apply node_lt_transitive. } 
-              inversion Hsort as [|? ? _ Hall]; subst.
-              apply node_rep_forall_app in Hall.
-              destruct Hall as [_ Hall].
-              inversion Hall as [|? ? Hfalse]; subst.
-              rewrite /node_lt in Hfalse.
-              assert (node_key tail = INT_MAX) by auto.
-              lia.
-            + inversion Hsplit_sep. 
-              by apply in_app_iff; right; right; left.
-            + apply in_app_iff in Hin.
-              destruct Hin as [|[|[]]]; first by eapply elem_of_list_In.
-              inversion Hsplit_sep. inversion Hcurr.
-              subst; exfalso.
-              rewrite -Hsplit_sep in Hsort.
-              do 2 apply node_rep_sorted_app in Hsort as (_ & Hsort).
-              apply Sorted_StronglySorted in Hsort; last first.
-              { unfold Relations_1.Transitive; apply node_lt_transitive. } 
-              inversion Hsort as [|? ? _ Hall]; subst.
-              apply node_rep_forall_app in Hall.
-              destruct Hall as [_ Hall].
-              inversion Hall as [|? ? Hfalse]; subst.
-              rewrite /node_lt in Hfalse.
-              assert (node_key tail = INT_MAX) by auto.
-              lia.
-          }
-
-          iMod (own_update with "Hown_auth") as "[Hown_auth Hown_auth_frag]".
-          { apply auth_update_alloc, (gset_local_update_union _ _ {[ next ]}). }
-          assert (ε ∪ {[ next ]} = {[ next ]}) as -> by set_solver.
-          assert (S ∪ {[ next ]} = S) as -> by set_solver.
-        
-          rewrite (list_equiv_split curr next ([head] ++ L)); last first.
-          { rewrite app_ass -Hsplit_sep //. }
-          iDestruct "Hlist" as (l' γ) "(>%Hsome & Hpt & #Hlock & Himp)".
-          assert (l = l') as <- by congruence.
-
-          wp_load.
-          iPoseProof ("Himp" with "Hpt") as "Hlist".
-          iMod ("Hclose" with "[Hlist Hown_auth Hown_frac Hown_keys]") as "_".
-          { iNext; iExists S, Skeys, L; by iFrame. }
-
-          iModIntro. wp_let. wp_lam. wp_pures.
-          case_bool_decide as Hcase.
-          * exfalso.
-            assert (node_key next <= node_key pred); last by lia.
-
-            assert (In pred (next :: Lm)) as Hpred_in_m.
-            {
-              symmetry in Hsplit_sep.
-              rewrite Hsplit_sep //= in Hsort.
-              rewrite //= app_comm_cons in Hsplit_join.
-              rewrite -app_ass Hcurr app_ass Hsplit_join //= in Hsplit_sep.
-              apply sorted_node_lt_no_dup in Hsort.
-
-              destruct Lm as [|next' Lm] using rev_ind.
-              + left. eapply (no_dup_elem_unique (Ls ++ [curr]) L2 (Ls ++ L1) L2 succ).
-                { rewrite app_ass //=. }
-                rewrite app_ass //= app_ass //=.
-              + right. apply in_app_iff. right. left.
-                eapply (no_dup_elem_unique (Ls ++ [curr; next] ++ Lm) L2 (Ls ++ L1) L2 succ).
-                { rewrite app_ass //= in Hsort. rewrite app_ass //=. }
-                rewrite app_ass //= in Hsplit_sep.
-                rewrite //= app_ass app_ass //=.
-            }
-
+          rewrite -elem_of_elements -Hperm.
+          destruct Ls; assert (In next (L ++ [tail])) as Hin.
+          + inversion Hsplit_sep. by left.
+          + apply in_app_iff in Hin.
+            destruct Hin as [|[|[]]]; first by eapply elem_of_list_In.
+            inversion Hsplit_sep. inversion Hcurr.
+            subst; exfalso.
             rewrite -Hsplit_sep in Hsort.
             do 2 apply node_rep_sorted_app in Hsort as (_ & Hsort).
-            apply node_rep_sorted_app in Hsort as (Hsort & _).
-
             apply Sorted_StronglySorted in Hsort; last first.
             { unfold Relations_1.Transitive; apply node_lt_transitive. } 
-            inversion Hsort; subst. 
-            inversion Hpred_in_m; first by (subst; lia).
-            eapply node_lt_le_incl, Forall_forall; eauto.
-            rewrite elem_of_list_In //=.
-          * wp_if.
-            iApply ("IH" $! next with "[$] [$] [%]").
-            { lia. }
-
-            iNext; iApply "HΦ".
-      + iInv lazyN as (? ? L) "(>%Hperm & _ & _ & >Hown_auth & >Hown_frac & _ & Hlist)" "_".
-        iDestruct (own_valid_2 with "Hown_frac Hown_frag") 
-          as %->%frac_auth_agree_L.
-
-        iAssert ((⌜ curr = head ∨ In curr L ⌝)%I) with "[Hown_auth Hown_curr]" as %Hcurr_range.
-        {
-          iDestruct "Hown_curr" as "[Heq|Hown]"; first by iLeft.
-          iDestruct (own_valid_2 with "Hown_auth Hown") 
-            as %[Hvalid%gset_included]%auth_both_valid_discrete.
-          iPureIntro; right. 
-          rewrite -elem_of_list_In Hperm elem_of_elements.
-          set_solver.
+            inversion Hsort as [|? ? _ Hall]; subst.
+            apply node_rep_forall_app in Hall.
+            destruct Hall as [_ Hall].
+            inversion Hall as [|? ? Hfalse]; subst.
+            rewrite /node_lt in Hfalse.
+            assert (node_key tail = INT_MAX) by auto.
+            lia.
+          + inversion Hsplit_sep. 
+            by apply in_app_iff; right; right; left.
+          + apply in_app_iff in Hin.
+            destruct Hin as [|[|[]]]; first by eapply elem_of_list_In.
+            inversion Hsplit_sep. inversion Hcurr.
+            subst; exfalso.
+            rewrite -Hsplit_sep in Hsort.
+            do 2 apply node_rep_sorted_app in Hsort as (_ & Hsort).
+            apply Sorted_StronglySorted in Hsort; last first.
+            { unfold Relations_1.Transitive; apply node_lt_transitive. } 
+            inversion Hsort as [|? ? _ Hall]; subst.
+            apply node_rep_forall_app in Hall.
+            destruct Hall as [_ Hall].
+            inversion Hall as [|? ? Hfalse]; subst.
+            rewrite /node_lt in Hfalse.
+            assert (node_key tail = INT_MAX) by auto.
+            lia.
         }
 
-        rewrite (list_equiv_invert); last done.
-        iDestruct "Hlist" as (? ? ?) "(_ & >%Hsome & _ & _ & _)".
-        congruence.
+        iMod (own_update with "Hown_auth") as "[Hown_auth Hown_auth_frag]".
+        { apply auth_update_alloc, (gset_local_update_union _ _ {[ next ]}). }
+        assert (ε ∪ {[ next ]} = {[ next ]}) as -> by set_solver.
+        assert (S ∪ {[ next ]} = S) as -> by set_solver.
+      
+        rewrite (list_equiv_split curr next ([head] ++ L)); last first.
+        { rewrite app_ass -Hsplit_sep //. }
+        iDestruct "Hlist" as (γ) "(Hpt & #Hlock & Himp)".
+
+        wp_load.
+        iPoseProof ("Himp" with "Hpt") as "Hlist".
+        iMod ("Hclose" with "[Hlist Hown_auth Hown_frac Hown_keys]") as "_".
+        { iNext; iExists S, Skeys, L; by iFrame. }
+
+        iModIntro. wp_let. wp_lam. wp_pures.
+        case_bool_decide as Hcase.
+        * exfalso.
+          assert (node_key next <= node_key pred); last by lia.
+
+          assert (In pred (next :: Lm)) as Hpred_in_m.
+          {
+            symmetry in Hsplit_sep.
+            rewrite Hsplit_sep //= in Hsort.
+            rewrite //= app_comm_cons in Hsplit_join.
+            rewrite -app_ass Hcurr app_ass Hsplit_join //= in Hsplit_sep.
+            apply sorted_node_lt_no_dup in Hsort.
+
+            destruct Lm as [|next' Lm] using rev_ind.
+            + left. eapply (no_dup_elem_unique (Ls ++ [curr]) L2 (Ls ++ L1) L2 succ).
+              { rewrite app_ass //=. }
+              rewrite app_ass //= app_ass //=.
+            + right. apply in_app_iff. right. left.
+              eapply (no_dup_elem_unique (Ls ++ [curr; next] ++ Lm) L2 (Ls ++ L1) L2 succ).
+              { rewrite app_ass //= in Hsort. rewrite app_ass //=. }
+              rewrite app_ass //= in Hsplit_sep.
+              rewrite //= app_ass app_ass //=.
+          }
+
+          rewrite -Hsplit_sep in Hsort.
+          do 2 apply node_rep_sorted_app in Hsort as (_ & Hsort).
+          apply node_rep_sorted_app in Hsort as (Hsort & _).
+
+          apply Sorted_StronglySorted in Hsort; last first.
+          { unfold Relations_1.Transitive; apply node_lt_transitive. } 
+          inversion Hsort; subst. 
+          inversion Hpred_in_m; first by (subst; lia).
+          eapply node_lt_le_incl, Forall_forall; eauto.
+          rewrite elem_of_list_In //=.
+        * wp_if.
+          iApply ("IH" $! next with "[$] [$] [%]").
+          { lia. }
+
+          iNext; iApply "HΦ".
     Qed.
 
     Theorem contains_spec (key: Z) (v: val) (S: gset Z) (Γ: lazy_gname)
@@ -239,13 +219,13 @@ Module ContainsSpec (Params: LAZY_LIST_PARAMS).
     Proof.
       iIntros (Φ) "H HΦ".
       iDestruct "H" as (h head) "(%Hv & Hpt & %Hmin & Hown & #Hinv)".
-      wp_lam. wp_let. rewrite -Hv. wp_load.
+      wp_lam. wp_let. rewrite -Hv. wp_load. wp_let.
 
       wp_apply (find_spec with "[Hown]").
       { iFrame "# ∗". iSplit. by iLeft. iPureIntro; lia. }
 
       iIntros (pred succ) "(Hown & %Hkey_in_S)".
-      wp_let. wp_match. wp_pures. wp_lam. wp_pures.
+      wp_pures. wp_lam. wp_pures.
 
       iModIntro; case_bool_decide.
       + iApply "HΦ". iSplit. 
